PyDict.fst
@@ -8,26 +8,77 @@ open PyList
 
 
 (*
- - Note: Dictionaries are not fully supported yet
+   - Return true if k is hashable
 *)
-
-
-
 let is_hashable_key (k: pyTyp) = false
 
 (*
-  - Returns true if k 
+  - Returns true if each element in kl is hashable
 *)
 let rec is_hashable (kl: list pyTyp) = 
   match kl with
   | [] -> true
-  | k::kl' -> (is_hashable_key k) || (is_hashable kl')
+  | k::kl' -> (is_hashable_key k) && (is_hashable kl')
 
 let createDict (kvl: list (pyTyp * pyTyp)) = 
   let kl, vl = List.Tot.Base.unzip kvl in
   match is_hashable kl with
   | false -> ERR("Key is mot hashable")
   | true ->
+
+    let contains =
+      Map.upd emptyMap "__contains__" 
+        (BINFUN (fun (a, b) ->
+          match a with
+          | OBJ(obja) -> 
+            (match Map.sel (obja.fields) "keys" with
+            | PYTYP(objakl) ->
+              (match pyTypTobuiltins objakl with
+              | LIST(kl) -> BOOL(list_contains kl b)
+              | _ -> NONE)
+            | _ -> NONE )  
+          | _ -> NONE)) in
+
+    let lt =
+    Map.upd contains "__lt__" 
+      (BINFUN (fun (a, b) ->  NONE)) in
+        
+    let le =
+      Map.upd lt "__le__" 
+        (BINFUN (fun (a, b) -> NONE)) in
+    
+    let eq =
+      Map.upd le "__eq__" 
+        (BINFUN (fun (a, b) -> 
+          match (pyTypTobuiltins a, pyTypTobuiltins b) with 
+          | DICT(kvl1), DICT(kvl2) ->
+            let kvl1_keys, kvl1_vals = List.Tot.Base.unzip kvl1 in
+            let kvl2_keys, kvl2_vals = List.Tot.Base.unzip kvl2 in
+            (match list_lex_eq kvl1_keys kvl2_keys, list_lex_eq kvl1_vals kvl2_vals with
+            | BOOL(b1), BOOL(b2) -> BOOL(b1 && b2)
+            | _ -> BOOL(false))  
+          | _ -> NONE)) in
+
+    let neq =
+      Map.upd eq "__ne__" 
+        (BINFUN (fun (a, b) -> 
+          match (pyTypTobuiltins a, pyTypTobuiltins b) with 
+          | DICT(kvl1), DICT(kvl2) ->
+            let kvl1_keys, kvl1_vals = List.Tot.Base.unzip kvl1 in
+            let kvl2_keys, kvl2_vals = List.Tot.Base.unzip kvl2 in
+            (match list_lex_ne kvl1_keys kvl2_keys, list_lex_ne kvl1_vals kvl2_vals with
+            | BOOL(b1), BOOL(b2) -> BOOL(b1 && b2)
+            | _ -> BOOL(false))  
+          | _ -> NONE)) in
+
+    let gt =
+      Map.upd neq "__gt__" 
+        (BINFUN (fun (a, b) -> NONE)) in
+
+    let ge =
+      Map.upd gt "__ge__" 
+        (BINFUN (fun (a, b) -> NONE)) in
+
     let keys = Map.upd emptyMap "keys" (createList kl) in
     let values = Map.upd keys "values" (createList vl) in
     let obj: type0 = {
@@ -38,4 +89,3 @@ let createDict (kvl: list (pyTyp * pyTyp)) =
       methods = emptyMap 
     } in
     PYTYP(OBJ(obj))
-
